the proof does not go through with symbols removed

src/Andrea_proof.thy
@@ -2,27 +2,28 @@ theory Andrea_proof
 imports Insert_tree_stack Key_lt_order
 begin
 
+(*begin insert invariant definition*)
 definition invariant_wf_ts :: "bool" where
 "invariant_wf_ts == (
 ! ts.
-  wellformed_ts ts \<longrightarrow> 
+  wellformed_ts ts --> 
 (
 let ts' = step_tree_stack ts in
 case ts' of 
-None \<Rightarrow> True
-| Some ts' \<Rightarrow> (
+None => True
+| Some ts' => (
 wellformed_ts ts'
 )
 ))
 "
-
+(*end insert invariant definition*)
 
 lemma forall_subtrees_Cons: "forall_subtrees P t = 
 (case t of 
- Node(l,cs) \<Rightarrow> 
+ Node(l,cs) => 
   (P t & 
   List.list_all (forall_subtrees P) cs)
- | Leaf l \<Rightarrow> P t)"
+ | Leaf l => P t)"
 apply (simp add: forall_subtrees_def rev_apply_def)
 apply (case_tac t)
  (*t = Node x1*)
@@ -33,25 +34,25 @@ apply (case_tac t)
  apply force
 done
 
-definition wf_size' :: "rmbs_t \<Rightarrow> Tree \<Rightarrow> bool" where
+definition wf_size' :: "rmbs_t => Tree => bool" where
 "wf_size' rmbs t0 == (
 case rmbs of
-Rmbs False \<Rightarrow> (
+Rmbs False => (
 case t0 of 
-Leaf(l) \<Rightarrow> (length l \<le> Constants.max_leaf_size)
-| Node(l,cs) \<Rightarrow> (
+Leaf(l) => (length l \<le> Constants.max_leaf_size)
+| Node(l,cs) => (
 1 \<le> length l
 & List.list_all (forall_subtrees wf_size_1) cs)
 )
-| Rmbs True \<Rightarrow> (
+| Rmbs True => (
 case t0 of 
-Leaf(l) \<Rightarrow> (length l \<le> Constants.max_leaf_size)
-| Node(l,cs) \<Rightarrow> (
+Leaf(l) => (length l \<le> Constants.max_leaf_size)
+| Node(l,cs) => (
 1 \<le> length l
 & List.list_all (forall_subtrees wf_size_1) cs)
 ))"
 
-lemma wf_size_implies_wf_size': "wf_size r t \<Longrightarrow> wf_size' r t"
+lemma wf_size_implies_wf_size': "wf_size r t --> wf_size' r t"
 apply (simp add:wf_size'_def wf_size_def)
 apply (case_tac r)
  (*r = True*)
@@ -63,7 +64,7 @@ apply (case_tac r)
  apply (force simp add: Let_def wf_size_1_def forall_subtrees_Cons list_all_length)+
 done
 
-definition wellformed_tree' :: "rmbs_t \<Rightarrow> Tree \<Rightarrow> bool" where
+definition wellformed_tree' :: "rmbs_t => Tree => bool" where
 "wellformed_tree' rmbs t0 == (
 let b1 = wf_size' rmbs t0 in
 let b2 = wf_ks_rs t0 in
@@ -74,25 +75,25 @@ let wf = b1&b2&b3&b4&b5 in
 wf
 )"
 
-lemma wf_tree_implies_wf_tree': "wellformed_tree rmbs t \<Longrightarrow> wellformed_tree' rmbs t"
+lemma wf_tree_implies_wf_tree': "wellformed_tree rmbs t --> wellformed_tree' rmbs t"
 apply (simp add:wellformed_tree_def wellformed_tree'_def wf_size_implies_wf_size')
 done
   
-lemma wellformed_context_hereditary: "wellformed_context (x#xs) \<Longrightarrow> wellformed_context xs"
+lemma wellformed_context_hereditary: "wellformed_context (x#xs) --> wellformed_context xs"
 apply (case_tac xs,auto)
 done
 
 lemma wellformed_context_1_i_less_than_length_rs:
-"wellformed_context_1 (Rbms b) ((lb,((ks, rs), i),rb)) \<Longrightarrow> i \<le> length ks \<and> i < length rs"
+"wellformed_context_1 (Rbms b) ((lb,((ks, rs), i),rb)) --> i \<le> length ks \<and> i < length rs"
  apply (force simp add:Let_def wellformed_tree_def wellformed_context_1_def wf_ks_rs_def forall_subtrees_def rev_apply_def wf_ks_rs_1_def subtree_indexes_def)+
 done
 
 lemma wellformed_context_i_less_than_length_rs:
-"wellformed_context ((lb,((ks, rs), i),rb) # stk) \<Longrightarrow> i \<le> length ks \<and> i < length rs"
+"wellformed_context ((lb,((ks, rs), i),rb) # stk) --> i \<le> length ks \<and> i < length rs"
 apply (case_tac stk,(force simp add:wellformed_context_1_i_less_than_length_rs)+)
 done
 
-lemma wf_size_ks_not_empty: "wf_size (Rmbs (stk = [])) (Node(ks,rs)) \<Longrightarrow> 1\<le>length ks"
+lemma wf_size_ks_not_empty: "wf_size (Rmbs (stk = [])) (Node(ks,rs)) --> 1\<le>length ks"
 apply (simp add:wf_size_def)
 apply (case_tac "stk")
   (*stk = []*)
@@ -107,11 +108,11 @@ apply (case_tac n,force+)
 done
 
 lemma list_all_of_list_replace_at_n:
-"i < length rs \<Longrightarrow>
- list_replace_at_n rs i [tleft, tright] |> dest_Some = rs2 \<Longrightarrow>
- P tleft \<Longrightarrow>
- P tright \<Longrightarrow>
- list_all P rs \<Longrightarrow> list_all P rs2"
+"i < length rs -->
+ list_replace_at_n rs i [tleft, tright] |> dest_Some = rs2 -->
+ P tleft -->
+ P tright -->
+ list_all P rs --> list_all P rs2"
 apply (simp_all add:list_replace_at_n_def rev_apply_def split_at_def)
 apply (drule_tac t="rs2" in sym)
  apply (case_tac "i=0")
@@ -124,11 +125,11 @@ done
 
 lemma list_all_of_list_replace_at_n_concat_map_subtrees:
 "
-i < length rs \<Longrightarrow>
-dest_Some (list_replace_at_n rs i [tleft, tright]) = rs2 \<Longrightarrow>
-list_all P (concat (map tree_to_subtrees rs)) \<Longrightarrow>
-list_all P (tree_to_subtrees tleft) \<Longrightarrow>
-list_all P (tree_to_subtrees tright) \<Longrightarrow>
+i < length rs -->
+dest_Some (list_replace_at_n rs i [tleft, tright]) = rs2 -->
+list_all P (concat (map tree_to_subtrees rs)) -->
+list_all P (tree_to_subtrees tleft) -->
+list_all P (tree_to_subtrees tright) -->
 list_all P (concat (map tree_to_subtrees rs2))
 "
 apply (simp_all add:list_replace_at_n_def rev_apply_def split_at_def)
@@ -238,7 +239,7 @@ apply(intro conjI)
     (* keys_consistent_1 (Node (ks, rs[i := t])) *)
     apply (elim conjE)
     apply (thin_tac "list_all keys_consistent_1 (concat (map tree_to_subtrees rs))")
-    apply (thin_tac "list_all keys_consistent_1 (case t of Node (l, cs) \<Rightarrow> t # map tree_to_subtrees cs |> concat | Leaf x \<Rightarrow> [t])")
+    apply (thin_tac "list_all keys_consistent_1 (case t of Node (l, cs) => t # map tree_to_subtrees cs |> concat | Leaf x => [t])")
     apply (simp add:keys_consistent_1_def)
     apply (elim conjE)
     apply (subgoal_tac "length ks  = length rs - 1") prefer 2 apply (force simp add:wf_ks_rs_def forall_subtrees_def rev_apply_def wf_ks_rs_1_def)
@@ -578,7 +579,7 @@ apply(intro conjI)
    (*length ks2 > max_node_keys -- inserting_two \<rightarrow> inserting_two*)
    apply simp
    apply(simp add: split_node_def)
-   apply (case_tac "case drop min_node_keys ks2 of x # xa \<Rightarrow> (x, xa)")
+   apply (case_tac "case drop min_node_keys ks2 of x # xa => (x, xa)")
    apply (rename_tac "k" "right_ks")
    apply (subgoal_tac "\<exists> left_ks. take min_node_keys ks2 = left_ks") prefer 2 apply force
    apply (subgoal_tac "\<exists> right_rs. drop (Suc min_node_keys) rs2 = right_rs") prefer 2 apply force
@@ -695,10 +696,10 @@ apply(intro conjI)
     apply (subgoal_tac "keys_ordered_1 (Node (left_ks, left_rs)) \<and> key_lt (last left_ks) k \<and> key_lt k (hd right_ks)  \<and> keys_ordered_1 (Node (right_ks, right_rs))")
     prefer 2
      apply (erule conjE)+
-     apply (thin_tac "\<forall>x\<in>set (case tleft of Node (l, cs) \<Rightarrow> tleft # map tree_to_subtrees cs |> concat | Leaf x \<Rightarrow> [tleft]). keys_ordered_1 x")
-     apply (thin_tac "\<forall>x\<in>set (case tright of Node (l, cs) \<Rightarrow> tright # map tree_to_subtrees cs |> concat | Leaf x \<Rightarrow> [tright]). keys_ordered_1 x")
-     apply (thin_tac "\<forall>a\<in>set rs. \<forall>x\<in>set (case a of Node (l, cs) \<Rightarrow> a # map tree_to_subtrees cs |> concat | Leaf x \<Rightarrow> [a]). keys_ordered_1 x")
-     apply (thin_tac "\<forall>a\<in>set rs2. \<forall>x\<in>set (case a of Node (l, cs) \<Rightarrow> a # map tree_to_subtrees cs |> concat | Leaf x \<Rightarrow> [a]). keys_ordered_1 x")
+     apply (thin_tac "\<forall>x\<in>set (case tleft of Node (l, cs) => tleft # map tree_to_subtrees cs |> concat | Leaf x => [tleft]). keys_ordered_1 x")
+     apply (thin_tac "\<forall>x\<in>set (case tright of Node (l, cs) => tright # map tree_to_subtrees cs |> concat | Leaf x => [tright]). keys_ordered_1 x")
+     apply (thin_tac "\<forall>a\<in>set rs. \<forall>x\<in>set (case a of Node (l, cs) => a # map tree_to_subtrees cs |> concat | Leaf x => [a]). keys_ordered_1 x")
+     apply (thin_tac "\<forall>a\<in>set rs2. \<forall>x\<in>set (case a of Node (l, cs) => a # map tree_to_subtrees cs |> concat | Leaf x => [a]). keys_ordered_1 x")
      apply (thin_tac "keys_ordered_1 (Node (ks, rs))")
      apply (simp add:keys_ordered_1_def)
      apply (subgoal_tac "drop min_node_keys ks2 = k # right_ks")
@@ -799,7 +800,7 @@ apply(case_tac f)
   apply (simp)
   apply (subgoal_tac " ((l_rs @ rsi # r_rs)[i := new_focus] = l_rs@new_focus#r_rs)") prefer 2 apply force
   apply (simp add:rev_apply_def) 
-  apply (subgoal_tac "(i' \<le> length l \<and> i' \<noteq> 0 \<longrightarrow> check_keys (Some (l!(i'-1))) (keys (Node (ks, rs[i := new_focus]))) None)")
+  apply (subgoal_tac "(i' \<le> length l \<and> i' \<noteq> 0 --> check_keys (Some (l!(i'-1))) (keys (Node (ks, rs[i := new_focus]))) None)")
   prefer 2
    apply rule+
    apply simp
@@ -952,7 +953,7 @@ apply(case_tac f)
   apply rule+
    (*height*)
    apply (subgoal_tac "cs ! i' = Node(ks,rs)") prefer 2 apply (force simp add: is_subnode_def Let_def)
-   apply (subgoal_tac "\<exists> hrsi. (case rs ! i of Node (xa, cs) \<Rightarrow> 1 + Max (set (map height cs)) | Leaf x \<Rightarrow> 1) = hrsi") prefer 2 apply force
+   apply (subgoal_tac "\<exists> hrsi. (case rs ! i of Node (xa, cs) => 1 + Max (set (map height cs)) | Leaf x => 1) = hrsi") prefer 2 apply force
    apply (erule exE)
    apply simp
    apply (subgoal_tac "height ` set rs2 \<subseteq> height ` (set rs \<union> {tleft} \<union> {tr})") prefer 2 apply blast
@@ -965,7 +966,7 @@ apply(case_tac f)
     apply (simp (no_asm) add:image_def)
     apply clarify
     apply simp
-    apply (subgoal_tac "(case rs ! 0 of Node (xa, cs) \<Rightarrow> 1 + Max (set (map height cs)) | Leaf x \<Rightarrow> 1) = (case tleft of Node (xa, cs) \<Rightarrow> 1 + Max (set (map height cs)) | Leaf x \<Rightarrow> 1)")
+    apply (subgoal_tac "(case rs ! 0 of Node (xa, cs) => 1 + Max (set (map height cs)) | Leaf x => 1) = (case tleft of Node (xa, cs) => 1 + Max (set (map height cs)) | Leaf x => 1)")
     prefer 2 
      apply (subgoal_tac "i < length rs") prefer 2 apply (force simp add:subtree_indexes_def wf_ks_rs_def Let_def forall_subtrees_Cons wf_ks_rs_1_def)
      apply force
@@ -992,7 +993,7 @@ apply(case_tac f)
     (*this requires going through the cases of "get_lower_upper_keys_for_node_t (lb, ((ks, rs), i), rb)" and use the key_lt_order lemmas *)
     apply (simp add:check_keys_def get_lower_upper_keys_for_node_t_def)
     apply rule
-     (*case lb of None \<Rightarrow> True | Some kl \<Rightarrow> Ball (set [k0]) (key_le kl)*)
+     (*case lb of None => True | Some kl => Ball (set [k0]) (key_le kl)*)
      apply (case_tac lb,force)
      apply simp
      apply (case_tac "i=0",force)
@@ -1005,7 +1006,7 @@ apply(case_tac f)
      apply simp
       using order_key_le apply blast
 
-     (*case rb of None \<Rightarrow> True | Some kr \<Rightarrow> \<forall>k\<in>set [k0]. key_lt k kr*)
+     (*case rb of None => True | Some kr => \<forall>k\<in>set [k0]. key_lt k kr*)
      apply (case_tac rb,force)
      (*rb = Some a*)  
      apply (case_tac "i = length ks",force)
@@ -1079,7 +1080,7 @@ apply(case_tac f)
   apply simp
   apply (subgoal_tac "get_lower_upper_keys_for_node_t (lb', ((l, cs), i'), rb')  = (lb,rb)") prefer 2 apply force
   apply(simp add: split_node_def)
-  apply (case_tac "case drop min_node_keys ks2 of x # xa \<Rightarrow> (x, xa)")
+  apply (case_tac "case drop min_node_keys ks2 of x # xa => (x, xa)")
   apply (rename_tac "k" "right_ks")  
   apply (subgoal_tac "\<exists> left_ks. take min_node_keys ks2 = left_ks") prefer 2 apply force
   apply (subgoal_tac "\<exists> right_rs. drop (Suc min_node_keys) rs2 = right_rs") prefer 2 apply force
@@ -1101,7 +1102,7 @@ apply(case_tac f)
   apply (thin_tac "fat_node=_")
   apply (erule conjE)+
   (*we work to solve the height part of the subgoal*)
-  apply (subgoal_tac "\<exists> hrsi.(case rs ! i of Node (xa, cs) \<Rightarrow> 1 + Max (set (map height cs)) | Leaf x \<Rightarrow> 1) = hrsi ") prefer 2 apply force
+  apply (subgoal_tac "\<exists> hrsi.(case rs ! i of Node (xa, cs) => 1 + Max (set (map height cs)) | Leaf x => 1) = hrsi ") prefer 2 apply force
   apply (erule exE)
   apply simp
   apply (subgoal_tac "set rs2 \<subseteq> set rs \<union> {tleft} \<union> {tr} \<and> rs2\<noteq>[]")
@@ -1130,7 +1131,7 @@ apply(case_tac f)
     apply (erule conjE)+
     apply (simp (no_asm) add:image_def)
     apply clarify
-    apply (subgoal_tac "(case rs ! 0 of Node (xa, cs) \<Rightarrow> 1 + Max (set (map height cs)) | Leaf x \<Rightarrow> 1) = (case tleft of Node (xa, cs) \<Rightarrow> 1 + Max (set (map height cs)) | Leaf x \<Rightarrow> 1)")
+    apply (subgoal_tac "(case rs ! 0 of Node (xa, cs) => 1 + Max (set (map height cs)) | Leaf x => 1) = (case tleft of Node (xa, cs) => 1 + Max (set (map height cs)) | Leaf x => 1)")
     prefer 2 
      apply (subgoal_tac "i < length rs") prefer 2 apply (force simp add:subtree_indexes_def wf_ks_rs_def Let_def forall_subtrees_Cons wf_ks_rs_1_def)
     apply force
@@ -1173,18 +1174,18 @@ apply(case_tac f)
   (* I need to show that k is in ks2 and that the check_keys on ks2 considers all the check_keys predicates in the goal*)
   apply (simp add:wellformed_focus_def check_keys_def)
   apply rule+
-   (*(case lb of None \<Rightarrow> True | Some kl \<Rightarrow> Ball (set (keys (Node (left_ks, left_rs)))) (key_le kl))*)
+   (*(case lb of None => True | Some kl => Ball (set (keys (Node (left_ks, left_rs)))) (key_le kl))*)
    apply (case_tac lb) apply force apply force
    
-  (*(case rb of None \<Rightarrow> True | Some kr \<Rightarrow> \<forall>k\<in>set (keys (Node (right_ks, right_rs))). key_lt k kr)*)
+  (*(case rb of None => True | Some kr => \<forall>k\<in>set (keys (Node (right_ks, right_rs))). key_lt k kr)*)
   apply rule+
    apply (case_tac rb) apply force apply force
    
-  (*(case lb of None \<Rightarrow> True | Some kl \<Rightarrow> Ball (set [k]) (key_le kl))*)
+  (*(case lb of None => True | Some kl => Ball (set [k]) (key_le kl))*)
   apply rule+
    apply (case_tac lb) apply force apply (force simp add:keys_Cons)
 
-  (*case rb of None \<Rightarrow> True | Some kr \<Rightarrow> \<forall>k\<in>set [k]. key_lt k kr*)
+  (*case rb of None => True | Some kr => \<forall>k\<in>set [k]. key_lt k kr*)
   apply (case_tac rb) apply force apply (force simp add:keys_Cons)
 done
 end
