src/Key_value.thy
@@ -5,7 +5,7 @@ begin
 typedecl key
 typedecl value_t
 
-consts key_lt :: "key \<Rightarrow> key \<Rightarrow> bool"
+consts key_lt :: "key => key => bool"
 
 definition key_le :: "key => key => bool" where
   "key_le k1 k2 == (k1 = k2) | (key_lt k1 k2)"
@@ -13,20 +13,21 @@ definition key_le :: "key => key => bool" where
 definition kv_lt :: "(key * value_t) => (key * value_t) => bool" where
   "kv_lt kv1 kv2 == (key_lt (fst kv1) (fst kv2))"
 
-
-definition check_keys :: "key option \<Rightarrow> key list \<Rightarrow> key option \<Rightarrow> bool" where
+(*begin check keys definition*)
+definition check_keys :: "key option => key list => key option => bool" where
 "check_keys kl ks kr == (
 let b1 = (
-case kl of None \<Rightarrow> True 
-| Some kl \<Rightarrow> (! k : set ks. key_le kl k)
+case kl of None => True 
+| Some kl => (! k : set ks. key_le kl k)
 )
 in
 let b2 = (
-case kr of None \<Rightarrow> True 
-| Some kr \<Rightarrow> (! k : set ks. key_lt k kr)
+case kr of None => True 
+| Some kr => (! k : set ks. key_lt k kr)
 )
 in
 b1 & b2
 )"
+(*end check keys definition*)
 
 end
